Update most of the taint analysis

vale/code/arch/x64/X64.Leakage_Ins.fst
@@ -58,7 +58,10 @@ let check_if_ins_consumes_fixed_time ins ts =
         end
    | S.Push src -> if Secret? (ts'.regTaint Rsp) || Secret? (operand_taint src ts' Public) then false, ts
      else fixedTime, ts'
-   | S.Pop dst -> if Secret? (ts'.regTaint Rsp) then false, ts else fixedTime, ts'
+   | S.Pop dst -> 
+     // Pop should be a public instruction
+     if Secret? (ts'.regTaint Rsp) || Secret? (ins.t) then false, ts 
+     else fixedTime, ts'
    | S.Adox64 _ _ -> false, ts (* Unhandled yet *)
    | S.Add64 _ _ | S.AddCarry64 _ _ | S.Adcx64 _ _  -> begin
           match dsts with
@@ -81,6 +84,11 @@ val lemma_public_flags_same: (ts:taintState) -> (ins:tainted_ins{S.Mul64? ins.i}
 publicFlagValuesAreSame ts s1 s2 ==> publicFlagValuesAreSame (snd (check_if_ins_consumes_fixed_time ins ts)) (taint_eval_ins ins s1) (taint_eval_ins ins s2))
 
 let lemma_public_flags_same ts ins = ()
+
+let frame_update_heap_x (ptr:int) (j:int) (v:nat64) (mem:S.heap) : Lemma
+  (requires j < ptr \/ j >= ptr + 8)
+  (ensures (let new_mem = S.update_heap64 ptr v mem in
+    mem.[j] == new_mem.[j])) = frame_update_heap ptr v mem
 
 let lemma_push_same_public_aux (ts:taintState) (ins:tainted_ins{S.Push? ins.i}) (s1:traceState) (s2:traceState)
                                (fuel:nat) (b:bool) (ts':taintState)
@@ -113,13 +121,13 @@ let lemma_push_same_public_aux (ts:taintState) (ins:tainted_ins{S.Push? ins.i}) 
         let s2b = S.run (S.check (taint_match_list srcs t s2.memTaint)) s2.state in
         if x < ptr1 || x >= ptr1 + 8 then (
           // If we're outside the modified area, nothing changed, the property still holds
-          frame_update_heap ptr1 v1 s1b.S.mem;
-          frame_update_heap ptr1 v2 s2b.S.mem
+          frame_update_heap_x ptr1 x v1 s1b.S.mem;
+          frame_update_heap_x ptr1 x v2 s2b.S.mem
         ) else (
           if Secret? t then ()
           else (
             Opaque_s.reveal_opaque S.get_heap_val64_def;
-            // If x is modified by Public values, values are identical
+            // If x is modified by Public values, values are identical            
             assert (v1 == v2);
             correct_update_get ptr1 v1 s1b.S.mem;
             correct_update_get ptr1 v2 s2b.S.mem;
@@ -137,101 +145,548 @@ let lemma_push_same_public (ts:taintState) (ins:tainted_ins{S.Push? ins.i}) (s1:
   = let b, ts' = check_if_ins_consumes_fixed_time ins ts in
     Classical.move_requires (lemma_push_same_public_aux ts ins s1 s2 fuel b) ts'
 
+let lemma_pop_same_public_aux (ts:taintState) (ins:tainted_ins{S.Pop? ins.i}) (s1:traceState) (s2:traceState)
+                               (fuel:nat) (b:bool) (ts':taintState)
+  :Lemma (requires ((b, ts') == check_if_ins_consumes_fixed_time ins ts /\ b /\
+                    is_explicit_leakage_free_lhs (Ins ins) fuel ts ts' s1 s2))
+         (ensures  (is_explicit_leakage_free_rhs (Ins ins) fuel ts ts' s1 s2)) =
+    let S.Pop dst, t = ins.i, ins.t in
+    let dsts, srcs = extract_operands ins.i in
 
-val lemma_pop_same_public: (ts:taintState) -> (ins:tainted_ins{let i, _, _ = ins.ops in S.Pop? i}) -> (s1:traceState) -> (s2:traceState) -> (fuel:nat) -> Lemma
-(let b, ts' = check_if_ins_consumes_fixed_time ins ts in
+    let r1 = taint_eval_code (Ins ins) fuel s1 in
+    let r2 = taint_eval_code (Ins ins) fuel s2 in
+
+    let s1' = Some?.v r1 in
+    let s2' = Some?.v r2 in
+
+    let op = OMem (MReg Rsp 0) in
+
+    let v1 = S.eval_operand op s1.state in
+    let v2 = S.eval_operand op s2.state in
+    let aux_value () : Lemma (v1 == v2) = Opaque_s.reveal_opaque S.get_heap_val64_def in
+    aux_value();
+
+    // We only need to help Z3 proving that public mem values are identical 
+    // after executing this instruction
+
+    let aux (x:int) : Lemma
+      (requires Public? s1'.memTaint.[x] || Public? s2'.memTaint.[x])
+      (ensures s1'.state.S.mem.[x] == s2'.state.S.mem.[x]) =
+        match dst with
+        | OConst _ | OReg _ -> ()
+        | OMem m -> begin
+        let ptr1 = S.eval_maddr m s1.state in
+        let ptr2 = S.eval_maddr m s2.state in
+        // Rsp is ensured to be Public if the taint analysis is successful
+        assert (ptr1 == ptr2);
+        // The instruction is executed after checking the taints of sources
+        let s1b = S.run (S.check (taint_match_list srcs t s1.memTaint)) s1.state in
+        let s2b = S.run (S.check (taint_match_list srcs t s2.memTaint)) s2.state in
+        if x < ptr1 || x >= ptr1 + 8 then (
+          // If we're outside the modified area, nothing changed, the property still holds
+          frame_update_heap_x ptr1 x v1 s1b.S.mem;
+          frame_update_heap_x ptr1 x v2 s2b.S.mem
+        ) else (
+          if Secret? t then ()
+          else (
+            correct_update_get ptr1 v1 s1b.S.mem;
+            correct_update_get ptr1 v2 s2b.S.mem;
+            // If values are identical, the bytes also are identical
+            same_mem_get_heap_val ptr1 s1'.state.S.mem s2'.state.S.mem
+          )
+        )
+        end
+        
+    in Classical.forall_intro (Classical.move_requires aux)
+
+
+let lemma_pop_same_public (ts:taintState) (ins:tainted_ins{S.Pop? ins.i}) (s1:traceState) (s2:traceState) 
+  (fuel:nat)
+  :Lemma (let b, ts' = check_if_ins_consumes_fixed_time ins ts in
   (b2t b ==> isExplicitLeakageFreeGivenStates (Ins ins) fuel ts ts' s1 s2))
+  = let b, ts' = check_if_ins_consumes_fixed_time ins ts in
+    Classical.move_requires (lemma_pop_same_public_aux ts ins s1 s2 fuel b) ts'
 
-#reset-options "--initial_ifuel 2 --max_ifuel 2 --initial_fuel 4 --max_fuel 4 --z3rlimit 80"
+let lemma_mov_same_public_aux (ts:taintState) (ins:tainted_ins{S.Mov64? ins.i}) (s1:traceState) (s2:traceState)
+                               (fuel:nat) (b:bool) (ts':taintState)
+  :Lemma (requires ((b, ts') == check_if_ins_consumes_fixed_time ins ts /\ b /\
+                    is_explicit_leakage_free_lhs (Ins ins) fuel ts ts' s1 s2))
+         (ensures  (is_explicit_leakage_free_rhs (Ins ins) fuel ts ts' s1 s2)) =
+    let S.Mov64 dst src, t = ins.i, ins.t in
+    let dsts, srcs = extract_operands ins.i in
 
-let lemma_pop_same_public ts ins s1 s2 fuel =
-  let b, ts' = check_if_ins_consumes_fixed_time ins ts in
-  let S.Pop dst, _, _ = ins.ops in
-  let op = OMem (MReg Rsp 0) in
-  let v1 = eval_operand op s1.state in
-  let v2 = eval_operand op s2.state in
-  match dst with
-  | OConst _ -> ()
-  | OReg _ -> ()
-  | OMem m ->
-    let ptr1 = eval_maddr m s1.state in
-    let ptr2 = eval_maddr m s2.state in
-    if not (valid_mem64 ptr1 s1.state.mem) || not (valid_mem64 ptr2 s2.state.mem) || Secret?   (ts.regTaint Rsp) then ()
-    else begin
-    lemma_store_load_mem64 ptr1 v1 s1.state.mem;
-    lemma_store_load_mem64 ptr2 v2 s2.state.mem;
-    lemma_valid_store_mem64 ptr1 v1 s1.state.mem;
-    lemma_valid_store_mem64 ptr2 v2 s2.state.mem;
-    lemma_frame_store_mem64 ptr1 v1 s1.state.mem;
-    lemma_frame_store_mem64 ptr2 v2 s2.state.mem
+    let r1 = taint_eval_code (Ins ins) fuel s1 in
+    let r2 = taint_eval_code (Ins ins) fuel s2 in
+
+    let s1' = Some?.v r1 in
+    let s2' = Some?.v r2 in
+
+    let s1b = S.run (S.check (taint_match_list srcs t s1.memTaint)) s1.state in
+    let s2b = S.run (S.check (taint_match_list srcs t s2.memTaint)) s2.state in
+
+    let taint = sources_taint srcs ts ins.t in
+
+    let v1 = S.eval_operand src s1.state in
+    let v2 = S.eval_operand src s2.state in
+
+    let aux_value () : Lemma 
+      (requires Public? taint)
+      (ensures v1 == v2) = 
+      Opaque_s.reveal_opaque S.get_heap_val64_def 
+    in
+
+    match dst with
+    | OConst _ -> ()
+    | OReg r -> if Secret? taint then () else aux_value()
+    | OMem m -> begin
+      let aux (x:int) : Lemma
+        (requires Public? s1'.memTaint.[x] || Public? s2'.memTaint.[x])
+        (ensures s1'.state.S.mem.[x] == s2'.state.S.mem.[x]) =
+        let ptr1 = S.eval_maddr m s1.state in
+        let ptr2 = S.eval_maddr m s2.state in
+        assert (ptr1 == ptr2);
+        if x < ptr1 || x >= ptr1 + 8 then (
+          // If we're outside the modified area, nothing changed, the property still holds
+          frame_update_heap_x ptr1 x v1 s1b.S.mem;
+          frame_update_heap_x ptr1 x v2 s2b.S.mem
+        ) else (
+          if Secret? taint then ()
+          else (
+            aux_value();
+            correct_update_get ptr1 v1 s1b.S.mem;
+            correct_update_get ptr1 v2 s2b.S.mem;
+            // If values are identical, the bytes also are identical
+            same_mem_get_heap_val ptr1 s1'.state.S.mem s2'.state.S.mem
+          )
+        )
+      
+      in Classical.forall_intro (Classical.move_requires aux)
     end
 
-
-val lemma_mov_same_public: (ts:taintState) -> (ins:tainted_ins{let i, _, _ = ins.ops in S.Mov64? i}) -> (s1:traceState) -> (s2:traceState) -> (fuel:nat) -> Lemma
-(let b, ts' = check_if_ins_consumes_fixed_time ins ts in
+let lemma_mov_same_public (ts:taintState) (ins:tainted_ins{S.Mov64? ins.i}) (s1:traceState) (s2:traceState) 
+  (fuel:nat)
+  :Lemma (let b, ts' = check_if_ins_consumes_fixed_time ins ts in
   (b2t b ==> isExplicitLeakageFreeGivenStates (Ins ins) fuel ts ts' s1 s2))
+  = let b, ts' = check_if_ins_consumes_fixed_time ins ts in
+    Classical.move_requires (lemma_mov_same_public_aux ts ins s1 s2 fuel b) ts'
 
-let lemma_mov_same_public ts ins s1 s2 fuel =
-  let b, ts' = check_if_ins_consumes_fixed_time ins ts in
-  let i, dsts, srcs = ins.ops in
-  let r1 = taint_eval_ins ins s1 in
-  let r2 = taint_eval_ins ins s2 in
-  match dsts with
-    | [OConst _] -> ()
-    | [OReg _] ->  ()
-    | [OMem m] ->
-      let ptr1 = eval_maddr m s1.state in
-      let ptr2 = eval_maddr m s2.state in
-      match srcs with
-        | [src] ->
-          let v1 = eval_operand src s1.state in
-          let v2 = eval_operand src s2.state in
-          if not (valid_mem64 ptr1 s1.state.mem) || not (valid_mem64 ptr2 s2.state.mem) then ()
-          else begin
-          lemma_store_load_mem64 ptr1 v1 s1.state.mem;
-          lemma_store_load_mem64 ptr2 v2 s2.state.mem;
-          lemma_valid_store_mem64 ptr1 v1 s1.state.mem;
-          lemma_valid_store_mem64 ptr2 v2 s2.state.mem;
-          lemma_frame_store_mem64 ptr1 v1 s1.state.mem;
-          lemma_frame_store_mem64 ptr2 v2 s2.state.mem
-          end
+let lemma_add_same_public_aux (ts:taintState) (ins:tainted_ins{S.Add64? ins.i}) (s1:traceState) (s2:traceState)
+                               (fuel:nat) (b:bool) (ts':taintState)
+  :Lemma (requires ((b, ts') == check_if_ins_consumes_fixed_time ins ts /\ b /\
+                    is_explicit_leakage_free_lhs (Ins ins) fuel ts ts' s1 s2))
+         (ensures  (is_explicit_leakage_free_rhs (Ins ins) fuel ts ts' s1 s2)) =
+    let S.Add64 dst src, t = ins.i, ins.t in
+    let dsts, srcs = extract_operands ins.i in
 
-val lemma_add_same_public: (ts:taintState) -> (ins:tainted_ins{let i, _, _ = ins.ops in S.Add64? i}) -> (s1:traceState) -> (s2:traceState) -> (fuel:nat) -> Lemma
-(let b, ts' = check_if_ins_consumes_fixed_time ins ts in
+    let r1 = taint_eval_code (Ins ins) fuel s1 in
+    let r2 = taint_eval_code (Ins ins) fuel s2 in
+
+    let s1' = Some?.v r1 in
+    let s2' = Some?.v r2 in
+
+    let s1b = S.run (S.check (taint_match_list srcs t s1.memTaint)) s1.state in
+    let s2b = S.run (S.check (taint_match_list srcs t s2.memTaint)) s2.state in
+
+    let taint = sources_taint srcs ts ins.t in
+
+    let v11 = S.eval_operand dst s1.state in
+    let v12 = S.eval_operand src s1.state in
+    let v21 = S.eval_operand dst s2.state in
+    let v22 = S.eval_operand src s2.state in
+    let sum1 = v11 + v12 in
+    let sum2 = v21 + v22 in
+    let new_carry1 = sum1 >= pow2_64 in
+    let new_carry2 = sum2 >= pow2_64 in
+    let v1 = sum1 % pow2_64 in
+    let v2 = sum2 % pow2_64 in
+
+    let aux_value () : Lemma 
+      (requires Public? taint)
+      (ensures v1 == v2) = 
+      Opaque_s.reveal_opaque S.get_heap_val64_def 
+    in
+
+    let aux_carry () : Lemma 
+      (requires Public? taint)
+      (ensures new_carry1 == new_carry2) = 
+      Opaque_s.reveal_opaque S.get_heap_val64_def 
+    in
+
+
+    match dst with
+    | OConst _ -> ()
+    | OReg r -> if Secret? taint then () else aux_value()
+    | OMem m -> begin
+      let aux_cf () : Lemma (publicCfFlagValuesAreSame ts' s1' s2') =
+        if Secret? taint then () else aux_carry()
+      in let aux (x:int) : Lemma
+        (requires Public? s1'.memTaint.[x] || Public? s2'.memTaint.[x])
+        (ensures s1'.state.S.mem.[x] == s2'.state.S.mem.[x]) =
+        let ptr1 = S.eval_maddr m s1.state in
+        let ptr2 = S.eval_maddr m s2.state in
+        assert (ptr1 == ptr2);
+         if x < ptr1 || x >= ptr1 + 8 then (
+          // If we're outside the modified area, nothing changed, the property still holds
+          frame_update_heap_x ptr1 x v1 s1b.S.mem;
+          frame_update_heap_x ptr1 x v2 s2b.S.mem
+        ) else (
+          if Secret? taint then ()
+          else (
+            aux_value();
+            correct_update_get ptr1 v1 s1b.S.mem;
+            correct_update_get ptr1 v2 s2b.S.mem;
+            // If values are identical, the bytes also are identical
+            same_mem_get_heap_val ptr1 s1'.state.S.mem s2'.state.S.mem
+          )
+        )
+      
+      in Classical.forall_intro (Classical.move_requires aux); aux_cf()
+    end
+
+let lemma_add_same_public (ts:taintState) (ins:tainted_ins{S.Add64? ins.i}) (s1:traceState) (s2:traceState) 
+  (fuel:nat)
+  :Lemma (let b, ts' = check_if_ins_consumes_fixed_time ins ts in
   (b2t b ==> isExplicitLeakageFreeGivenStates (Ins ins) fuel ts ts' s1 s2))
+  = let b, ts' = check_if_ins_consumes_fixed_time ins ts in
+    Classical.move_requires (lemma_add_same_public_aux ts ins s1 s2 fuel b) ts'
 
-#reset-options "--initial_ifuel 2 --max_ifuel 2 --initial_fuel 4 --max_fuel 4 --z3rlimit 100"
-let lemma_add_same_public ts ins s1 s2 fuel =
-  let b, ts' = check_if_ins_consumes_fixed_time ins ts in
-  let i, dsts, srcs = ins.ops in
-  let r1 = taint_eval_ins ins s1 in
-  let r2 = taint_eval_ins ins s2 in
-  match dsts with
-    | [OConst _] -> ()
-    | [OReg _] ->  ()
-    | [OMem m] ->
-      let ptr1 = eval_maddr m s1.state in
-      let ptr2 = eval_maddr m s2.state in
-      match srcs with
-        | [src1; src2] ->
-          let v11 = eval_operand src1 s1.state in
-          let v12 = eval_operand src2 s1.state in
-          let v21 = eval_operand src1 s2.state in
-          let v22 = eval_operand src2 s2.state in
-          let v1 = (v11 + v12) % pow2_64 in
-          let v2 = (v21 + v22) % pow2_64 in
-          if not (valid_mem64 ptr1 s1.state.mem) || not (valid_mem64 ptr2 s2.state.mem) then ()
-          else begin
-           lemma_store_load_mem64 ptr1 v1 s1.state.mem;
-          lemma_store_load_mem64 ptr2 v2 s2.state.mem;
-          lemma_valid_store_mem64 ptr1 v1 s1.state.mem;
-          lemma_valid_store_mem64 ptr2 v2 s2.state.mem;
-          lemma_frame_store_mem64 ptr1 v1 s1.state.mem;
-          lemma_frame_store_mem64 ptr2 v2 s2.state.mem
-          end
+let lemma_addlea_same_public_aux (ts:taintState) (ins:tainted_ins{S.AddLea64? ins.i}) (s1:traceState) (s2:traceState)
+                               (fuel:nat) (b:bool) (ts':taintState)
+  :Lemma (requires ((b, ts') == check_if_ins_consumes_fixed_time ins ts /\ b /\
+                    is_explicit_leakage_free_lhs (Ins ins) fuel ts ts' s1 s2))
+         (ensures  (is_explicit_leakage_free_rhs (Ins ins) fuel ts ts' s1 s2)) =
+    let S.AddLea64 dst src1 src2, t = ins.i, ins.t in
+    let dsts, srcs = extract_operands ins.i in
+
+    let r1 = taint_eval_code (Ins ins) fuel s1 in
+    let r2 = taint_eval_code (Ins ins) fuel s2 in
+
+    let s1' = Some?.v r1 in
+    let s2' = Some?.v r2 in
+
+    let s1b = S.run (S.check (taint_match_list srcs t s1.memTaint)) s1.state in
+    let s2b = S.run (S.check (taint_match_list srcs t s2.memTaint)) s2.state in
+
+    let taint = sources_taint srcs ts ins.t in
+
+    let v11 = S.eval_operand src1 s1.state in
+    let v12 = S.eval_operand src2 s1.state in
+    let v21 = S.eval_operand src1 s2.state in
+    let v22 = S.eval_operand src2 s2.state in
+    let sum1 = v11 + v12 in
+    let sum2 = v21 + v22 in
+    let v1 = sum1 % pow2_64 in
+    let v2 = sum2 % pow2_64 in
+
+    let aux_value () : Lemma 
+      (requires Public? taint)
+      (ensures v1 == v2) = 
+      Opaque_s.reveal_opaque S.get_heap_val64_def 
+    in
+
+    match dst with
+    | OConst _ -> ()
+    | OReg r -> if Secret? taint then () else aux_value()
+    | OMem m -> begin
+      let aux (x:int) : Lemma
+        (requires Public? s1'.memTaint.[x] || Public? s2'.memTaint.[x])
+        (ensures s1'.state.S.mem.[x] == s2'.state.S.mem.[x]) =
+        let ptr1 = S.eval_maddr m s1.state in
+        let ptr2 = S.eval_maddr m s2.state in
+        assert (ptr1 == ptr2);
+         if x < ptr1 || x >= ptr1 + 8 then (
+          // If we're outside the modified area, nothing changed, the property still holds
+          frame_update_heap_x ptr1 x v1 s1b.S.mem;
+          frame_update_heap_x ptr1 x v2 s2b.S.mem
+        ) else (
+          if Secret? taint then ()
+          else (
+            aux_value();
+            correct_update_get ptr1 v1 s1b.S.mem;
+            correct_update_get ptr1 v2 s2b.S.mem;
+            // If values are identical, the bytes also are identical
+            same_mem_get_heap_val ptr1 s1'.state.S.mem s2'.state.S.mem
+          )
+        )
+      
+      in Classical.forall_intro (Classical.move_requires aux)
+    end
+
+let lemma_addlea_same_public (ts:taintState) (ins:tainted_ins{S.AddLea64? ins.i}) (s1:traceState) (s2:traceState) 
+  (fuel:nat)
+  :Lemma (let b, ts' = check_if_ins_consumes_fixed_time ins ts in
+  (b2t b ==> isExplicitLeakageFreeGivenStates (Ins ins) fuel ts ts' s1 s2))
+  = let b, ts' = check_if_ins_consumes_fixed_time ins ts in
+    Classical.move_requires (lemma_addlea_same_public_aux ts ins s1 s2 fuel b) ts'
+
+#set-options "--z3rlimit 250"
+
+let lemma_addcarry_same_public_aux (ts:taintState) (ins:tainted_ins{S.AddCarry64? ins.i}) (s1:traceState) (s2:traceState)
+                               (fuel:nat) (b:bool) (ts':taintState)
+  :Lemma (requires ((b, ts') == check_if_ins_consumes_fixed_time ins ts /\ b /\
+                    is_explicit_leakage_free_lhs (Ins ins) fuel ts ts' s1 s2))
+         (ensures  (is_explicit_leakage_free_rhs (Ins ins) fuel ts ts' s1 s2)) =
+    let S.AddCarry64 dst src, t = ins.i, ins.t in
+    let dsts, srcs = extract_operands ins.i in
+
+    let r1 = taint_eval_code (Ins ins) fuel s1 in
+    let r2 = taint_eval_code (Ins ins) fuel s2 in
+
+    let s1' = Some?.v r1 in
+    let s2' = Some?.v r2 in
+
+    let s1b = S.run (S.check (taint_match_list srcs t s1.memTaint)) s1.state in
+    let s2b = S.run (S.check (taint_match_list srcs t s2.memTaint)) s2.state in
+
+    let taint = sources_taint srcs ts ins.t in
+    let taint = merge_taint taint ts.cfFlagsTaint in
+
+    let v11 = S.eval_operand dst s1.state in
+    let v12 = S.eval_operand src s1.state in
+    let v21 = S.eval_operand dst s2.state in
+    let v22 = S.eval_operand src s2.state in
+    let c1 = if S.cf s1.state.S.flags then 1 else 0 in
+    let c2 = if S.cf s2.state.S.flags then 1 else 0 in    
+    let sum1 = v11 + v12 + c1 in
+    let sum2 = v21 + v22 + c2 in
+    let new_carry1 = sum1 >= pow2_64 in
+    let new_carry2 = sum2 >= pow2_64 in
+    let v1 = sum1 % pow2_64 in
+    let v2 = sum2 % pow2_64 in
+
+    let aux_value () : Lemma 
+      (requires Public? taint)
+      (ensures v1 == v2) =
+      Opaque_s.reveal_opaque S.get_heap_val64_def 
+    in
+
+    let aux_carry () : Lemma 
+      (requires Public? taint)
+      (ensures new_carry1 == new_carry2) =
+      Opaque_s.reveal_opaque S.get_heap_val64_def 
+    in
+
+    match dst with
+    | OConst _ -> ()
+    | OReg r -> if Secret? taint then () else aux_value()
+    | OMem m -> begin
+      let aux_cf () : Lemma (publicCfFlagValuesAreSame ts' s1' s2') =
+        if Secret? taint then () else aux_carry()    
+      in let aux (x:int) : Lemma
+        (requires Public? s1'.memTaint.[x] || Public? s2'.memTaint.[x])
+        (ensures s1'.state.S.mem.[x] == s2'.state.S.mem.[x]) =
+        let ptr1 = S.eval_maddr m s1.state in
+        let ptr2 = S.eval_maddr m s2.state in
+        assert (ptr1 == ptr2);
+        if x < ptr1 || x >= ptr1 + 8 then (
+          // If we're outside the modified area, nothing changed, the property still holds
+          frame_update_heap_x ptr1 x v1 s1b.S.mem;
+          frame_update_heap_x ptr1 x v2 s2b.S.mem
+        ) else (
+          if Secret? taint then ()
+          else (
+            aux_value();
+            correct_update_get ptr1 v1 s1b.S.mem;
+            correct_update_get ptr1 v2 s2b.S.mem;
+            // If values are identical, the bytes also are identical
+            same_mem_get_heap_val ptr1 s1'.state.S.mem s2'.state.S.mem
+          )
+        )
+      
+      in Classical.forall_intro (Classical.move_requires aux); aux_cf()
+    end
+
+let lemma_addcarry_same_public (ts:taintState) (ins:tainted_ins{S.AddCarry64? ins.i}) (s1:traceState) (s2:traceState) 
+  (fuel:nat)
+  :Lemma (let b, ts' = check_if_ins_consumes_fixed_time ins ts in
+  (b2t b ==> isExplicitLeakageFreeGivenStates (Ins ins) fuel ts ts' s1 s2))
+  = let b, ts' = check_if_ins_consumes_fixed_time ins ts in
+    Classical.move_requires (lemma_addcarry_same_public_aux ts ins s1 s2 fuel b) ts'
+
+#set-options "--z3rlimit 300"
+
+let lemma_adcx_same_public_aux (ts:taintState) (ins:tainted_ins{S.Adcx64? ins.i}) (s1:traceState) (s2:traceState)
+                               (fuel:nat) (b:bool) (ts':taintState)
+  :Lemma (requires ((b, ts') == check_if_ins_consumes_fixed_time ins ts /\ b /\
+                    is_explicit_leakage_free_lhs (Ins ins) fuel ts ts' s1 s2))
+         (ensures  (is_explicit_leakage_free_rhs (Ins ins) fuel ts ts' s1 s2)) =
+    let S.Adcx64 dst src, t = ins.i, ins.t in
+    let dsts, srcs = extract_operands ins.i in
+
+    let r1 = taint_eval_code (Ins ins) fuel s1 in
+    let r2 = taint_eval_code (Ins ins) fuel s2 in
+
+    let s1' = Some?.v r1 in
+    let s2' = Some?.v r2 in
+
+    let s1b = S.run (S.check (taint_match_list srcs t s1.memTaint)) s1.state in
+    let s2b = S.run (S.check (taint_match_list srcs t s2.memTaint)) s2.state in
+
+    let taint = sources_taint srcs ts ins.t in
+    let taint = merge_taint taint ts.cfFlagsTaint in
+
+    let v11 = S.eval_operand dst s1.state in
+    let v12 = S.eval_operand src s1.state in
+    let v21 = S.eval_operand dst s2.state in
+    let v22 = S.eval_operand src s2.state in
+    let c1 = if S.cf s1.state.S.flags then 1 else 0 in
+    let c2 = if S.cf s2.state.S.flags then 1 else 0 in    
+    let sum1 = v11 + v12 + c1 in
+    let sum2 = v21 + v22 + c2 in
+    let new_carry1 = sum1 >= pow2_64 in
+    let new_carry2 = sum2 >= pow2_64 in
+    let v1 = sum1 % pow2_64 in
+    let v2 = sum2 % pow2_64 in
+
+    let aux_value () : Lemma 
+      (requires Public? taint)
+      (ensures v1 == v2) =
+      Opaque_s.reveal_opaque S.get_heap_val64_def 
+    in
+
+    let aux_carry () : Lemma 
+      (requires Public? taint)
+      (ensures new_carry1 == new_carry2) =
+      Opaque_s.reveal_opaque S.get_heap_val64_def 
+    in
+
+    match dst with
+    | OConst _ -> ()
+    | OReg r -> if Secret? taint then () else aux_value()
+    | OMem m -> begin
+      let aux_cf () : Lemma (publicCfFlagValuesAreSame ts' s1' s2') =
+        if Secret? taint then () else aux_carry()    
+      in let aux (x:int) : Lemma
+        (requires Public? s1'.memTaint.[x] || Public? s2'.memTaint.[x])
+        (ensures s1'.state.S.mem.[x] == s2'.state.S.mem.[x]) =
+        let ptr1 = S.eval_maddr m s1.state in
+        let ptr2 = S.eval_maddr m s2.state in
+        assert (ptr1 == ptr2);
+        if x < ptr1 || x >= ptr1 + 8 then (
+          // If we're outside the modified area, nothing changed, the property still holds
+          frame_update_heap_x ptr1 x v1 s1b.S.mem;
+          frame_update_heap_x ptr1 x v2 s2b.S.mem
+        ) else (
+          if Secret? taint then ()
+          else (
+            aux_value();
+            correct_update_get ptr1 v1 s1b.S.mem;
+            correct_update_get ptr1 v2 s2b.S.mem;
+            // If values are identical, the bytes also are identical
+            same_mem_get_heap_val ptr1 s1'.state.S.mem s2'.state.S.mem
+          )
+        )
+      
+      in Classical.forall_intro (Classical.move_requires aux); aux_cf()
+    end
+
+let lemma_adcx_same_public (ts:taintState) (ins:tainted_ins{S.Adcx64? ins.i}) (s1:traceState) (s2:traceState) 
+  (fuel:nat)
+  :Lemma (let b, ts' = check_if_ins_consumes_fixed_time ins ts in
+  (b2t b ==> isExplicitLeakageFreeGivenStates (Ins ins) fuel ts ts' s1 s2))
+  = let b, ts' = check_if_ins_consumes_fixed_time ins ts in
+    Classical.move_requires (lemma_adcx_same_public_aux ts ins s1 s2 fuel b) ts'
+
+#set-options "--z3rlimit 80"
 
 
-val lemma_mulx_same_public: (ts:taintState) -> (ins:tainted_ins{let i, _, _ = ins.ops in S.Mulx64? i}) -> (s1:traceState) -> (s2:traceState) -> (fuel:nat) -> Lemma
+let lemma_sub_same_public_aux (ts:taintState) (ins:tainted_ins{S.Sub64? ins.i}) (s1:traceState) (s2:traceState)
+                               (fuel:nat) (b:bool) (ts':taintState)
+  :Lemma (requires ((b, ts') == check_if_ins_consumes_fixed_time ins ts /\ b /\
+                    is_explicit_leakage_free_lhs (Ins ins) fuel ts ts' s1 s2))
+         (ensures  (is_explicit_leakage_free_rhs (Ins ins) fuel ts ts' s1 s2)) =
+    let S.Sub64 dst src, t = ins.i, ins.t in
+    let dsts, srcs = extract_operands ins.i in
+
+    let r1 = taint_eval_code (Ins ins) fuel s1 in
+    let r2 = taint_eval_code (Ins ins) fuel s2 in
+
+    let s1' = Some?.v r1 in
+    let s2' = Some?.v r2 in
+
+    let s1b = S.run (S.check (taint_match_list srcs t s1.memTaint)) s1.state in
+    let s2b = S.run (S.check (taint_match_list srcs t s2.memTaint)) s2.state in
+
+    let taint = sources_taint srcs ts ins.t in
+
+    let v11 = S.eval_operand dst s1.state in
+    let v12 = S.eval_operand src s1.state in
+    let v21 = S.eval_operand dst s2.state in
+    let v22 = S.eval_operand src s2.state in
+    let v1 = (v11 - v12) % pow2_64 in
+    let v2 = (v21 - v22) % pow2_64 in
+
+    let aux_value () : Lemma 
+      (requires Public? taint)
+      (ensures v1 == v2) = 
+      Opaque_s.reveal_opaque S.get_heap_val64_def 
+    in
+
+    match dst with
+    | OConst _ -> ()
+    | OReg r -> if Secret? taint then () else aux_value()
+    | OMem m -> begin
+      let aux (x:int) : Lemma
+        (requires Public? s1'.memTaint.[x] || Public? s2'.memTaint.[x])
+        (ensures s1'.state.S.mem.[x] == s2'.state.S.mem.[x]) =
+        let ptr1 = S.eval_maddr m s1.state in
+        let ptr2 = S.eval_maddr m s2.state in
+        assert (ptr1 == ptr2);
+         if x < ptr1 || x >= ptr1 + 8 then (
+          // If we're outside the modified area, nothing changed, the property still holds
+          frame_update_heap_x ptr1 x v1 s1b.S.mem;
+          frame_update_heap_x ptr1 x v2 s2b.S.mem
+        ) else (
+          if Secret? taint then ()
+          else (
+            aux_value();
+            correct_update_get ptr1 v1 s1b.S.mem;
+            correct_update_get ptr1 v2 s2b.S.mem;
+            // If values are identical, the bytes also are identical
+            same_mem_get_heap_val ptr1 s1'.state.S.mem s2'.state.S.mem
+          )
+        )
+      
+      in Classical.forall_intro (Classical.move_requires aux)
+    end
+
+let lemma_sub_same_public (ts:taintState) (ins:tainted_ins{S.Sub64? ins.i}) (s1:traceState) (s2:traceState) 
+  (fuel:nat)
+  :Lemma (let b, ts' = check_if_ins_consumes_fixed_time ins ts in
+  (b2t b ==> isExplicitLeakageFreeGivenStates (Ins ins) fuel ts ts' s1 s2))
+  = let b, ts' = check_if_ins_consumes_fixed_time ins ts in
+    Classical.move_requires (lemma_sub_same_public_aux ts ins s1 s2 fuel b) ts'
+
+let lemma_mul_same_public_aux (ts:taintState) (ins:tainted_ins{S.Mul64? ins.i}) (s1:traceState) (s2:traceState)
+                               (fuel:nat) (b:bool) (ts':taintState)
+  :Lemma (requires ((b, ts') == check_if_ins_consumes_fixed_time ins ts /\ b /\
+                    is_explicit_leakage_free_lhs (Ins ins) fuel ts ts' s1 s2))
+         (ensures  (is_explicit_leakage_free_rhs (Ins ins) fuel ts ts' s1 s2)) =
+    lemma_public_flags_same ts ins;
+    Opaque_s.reveal_opaque S.get_heap_val64_def
+
+let lemma_mul_same_public (ts:taintState) (ins:tainted_ins{S.Mul64? ins.i}) (s1:traceState) (s2:traceState) 
+  (fuel:nat)
+  :Lemma (let b, ts' = check_if_ins_consumes_fixed_time ins ts in
+  (b2t b ==> isExplicitLeakageFreeGivenStates (Ins ins) fuel ts ts' s1 s2))
+  = let b, ts' = check_if_ins_consumes_fixed_time ins ts in
+    Classical.move_requires (lemma_mul_same_public_aux ts ins s1 s2 fuel b) ts'
+
+let lemma_mulx_same_public_aux (ts:taintState) (ins:tainted_ins{S.Mulx64? ins.i}) (s1:traceState) (s2:traceState)
+                               (fuel:nat) (b:bool) (ts':taintState)
+  :Lemma (requires ((b, ts') == check_if_ins_consumes_fixed_time ins ts /\ b /\
+                    is_explicit_leakage_free_lhs (Ins ins) fuel ts ts' s1 s2))
+         (ensures  (is_explicit_leakage_free_rhs (Ins ins) fuel ts ts' s1 s2)) =
+  admit() // TODO
+
+let lemma_mulx_same_public (ts:taintState) (ins:tainted_ins{S.Mulx64? ins.i}) (s1:traceState) (s2:traceState) 
+  (fuel:nat)
+  :Lemma (let b, ts' = check_if_ins_consumes_fixed_time ins ts in
+  (b2t b ==> isExplicitLeakageFreeGivenStates (Ins ins) fuel ts ts' s1 s2))
+  = let b, ts' = check_if_ins_consumes_fixed_time ins ts in
+    Classical.move_requires (lemma_mulx_same_public_aux ts ins s1 s2 fuel b) ts'
+
+(*val lemma_mulx_same_public: (ts:taintState) -> (ins:tainted_ins{let i, _, _ = ins.ops in S.Mulx64? i}) -> (s1:traceState) -> (s2:traceState) -> (fuel:nat) -> Lemma
 (let b, ts' = check_if_ins_consumes_fixed_time ins ts in
   (b2t b ==> isExplicitLeakageFreeGivenStates (Ins ins) fuel ts ts' s1 s2))
 
@@ -326,286 +781,75 @@ let lemma_mulx_same_public ts ins s1 s2 fuel =
       end
       end
     | _ -> ()
+*)
 
-val lemma_sub_same_public: (ts:taintState) -> (ins:tainted_ins{let i, _, _ = ins.ops in S.Sub64? i}) -> (s1:traceState) -> (s2:traceState) -> (fuel:nat) -> Lemma
-(let b, ts' = check_if_ins_consumes_fixed_time ins ts in
+
+let lemma_imul_same_public_aux (ts:taintState) (ins:tainted_ins{S.IMul64? ins.i}) (s1:traceState) (s2:traceState)
+                               (fuel:nat) (b:bool) (ts':taintState)
+  :Lemma (requires ((b, ts') == check_if_ins_consumes_fixed_time ins ts /\ b /\
+                    is_explicit_leakage_free_lhs (Ins ins) fuel ts ts' s1 s2))
+         (ensures  (is_explicit_leakage_free_rhs (Ins ins) fuel ts ts' s1 s2)) =
+    let S.IMul64 dst src, t = ins.i, ins.t in
+    let dsts, srcs = extract_operands ins.i in
+
+    let r1 = taint_eval_code (Ins ins) fuel s1 in
+    let r2 = taint_eval_code (Ins ins) fuel s2 in
+
+    let s1' = Some?.v r1 in
+    let s2' = Some?.v r2 in
+
+    let s1b = S.run (S.check (taint_match_list srcs t s1.memTaint)) s1.state in
+    let s2b = S.run (S.check (taint_match_list srcs t s2.memTaint)) s2.state in
+
+    let taint = sources_taint srcs ts ins.t in
+
+    let v11 = S.eval_operand dst s1.state in
+    let v12 = S.eval_operand src s1.state in
+    let v21 = S.eval_operand dst s2.state in
+    let v22 = S.eval_operand src s2.state in
+    let v1 = FStar.UInt.mul_mod #64 v11 v12 in
+    let v2 = FStar.UInt.mul_mod #64 v21 v22 in
+
+    let aux_value () : Lemma 
+      (requires Public? taint)
+      (ensures v1 == v2) = 
+      Opaque_s.reveal_opaque S.get_heap_val64_def 
+    in
+
+    match dst with
+    | OConst _ -> ()
+    | OReg r -> if Secret? taint then () else aux_value()
+    | OMem m -> begin
+      let aux (x:int) : Lemma
+        (requires Public? s1'.memTaint.[x] || Public? s2'.memTaint.[x])
+        (ensures s1'.state.S.mem.[x] == s2'.state.S.mem.[x]) =
+        let ptr1 = S.eval_maddr m s1.state in
+        let ptr2 = S.eval_maddr m s2.state in
+        assert (ptr1 == ptr2);
+         if x < ptr1 || x >= ptr1 + 8 then (
+          // If we're outside the modified area, nothing changed, the property still holds
+          frame_update_heap_x ptr1 x v1 s1b.S.mem;
+          frame_update_heap_x ptr1 x v2 s2b.S.mem
+        ) else (
+          if Secret? taint then ()
+          else (
+            aux_value();
+            correct_update_get ptr1 v1 s1b.S.mem;
+            correct_update_get ptr1 v2 s2b.S.mem;
+            // If values are identical, the bytes also are identical
+            same_mem_get_heap_val ptr1 s1'.state.S.mem s2'.state.S.mem
+          )
+        )
+      
+      in Classical.forall_intro (Classical.move_requires aux)
+    end
+
+let lemma_imul_same_public (ts:taintState) (ins:tainted_ins{S.IMul64? ins.i}) (s1:traceState) (s2:traceState) 
+  (fuel:nat)
+  :Lemma (let b, ts' = check_if_ins_consumes_fixed_time ins ts in
   (b2t b ==> isExplicitLeakageFreeGivenStates (Ins ins) fuel ts ts' s1 s2))
-
-let lemma_sub_same_public ts ins s1 s2 fuel =
-  let b, ts' = check_if_ins_consumes_fixed_time ins ts in
-  let i, dsts, srcs = ins.ops in
-  let r1 = taint_eval_ins ins s1 in
-  let r2 = taint_eval_ins ins s2 in
- match dsts with
-    | [OConst _] -> ()
-    | [OReg _] ->  ()
-    | [OMem m] ->
-      let ptr1 = eval_maddr m s1.state in
-      let ptr2 = eval_maddr m s2.state in
-      match srcs with
-        | [src1; src2] ->
-          let v11 = eval_operand src1 s1.state in
-          let v12 = eval_operand src2 s1.state in
-          let v21 = eval_operand src1 s2.state in
-          let v22 = eval_operand src2 s2.state in
-          let v1 = (v11 - v12) % pow2_64 in
-          let v2 = (v21 - v22) % pow2_64 in
-          if not (valid_mem64 ptr1 s1.state.mem) || not (valid_mem64 ptr2 s2.state.mem) then ()
-          else begin
-           lemma_store_load_mem64 ptr1 v1 s1.state.mem;
-          lemma_store_load_mem64 ptr2 v2 s2.state.mem;
-          lemma_valid_store_mem64 ptr1 v1 s1.state.mem;
-          lemma_valid_store_mem64 ptr2 v2 s2.state.mem;
-          lemma_frame_store_mem64 ptr1 v1 s1.state.mem;
-          lemma_frame_store_mem64 ptr2 v2 s2.state.mem
-          end
-
-val lemma_imul_same_public: (ts:taintState) -> (ins:tainted_ins{let i, _, _ = ins.ops in S.IMul64? i}) -> (s1:traceState) -> (s2:traceState) -> (fuel:nat) -> Lemma
-(let b, ts' = check_if_ins_consumes_fixed_time ins ts in
-  (b2t b ==> isExplicitLeakageFreeGivenStates (Ins ins) fuel ts ts' s1 s2))
-
-let lemma_imul_same_public ts ins s1 s2 fuel =
-  let b, ts' = check_if_ins_consumes_fixed_time ins ts in
-  let i, dsts, srcs = ins.ops in
-  let r1 = taint_eval_ins ins s1 in
-  let r2 = taint_eval_ins ins s2 in
- match dsts with
-    | [OConst _] -> ()
-    | [OReg _] ->  ()
-    | [OMem m] ->
-      let ptr1 = eval_maddr m s1.state in
-      let ptr2 = eval_maddr m s2.state in
-      match srcs with
-        | [src1; src2] ->
-          let v11 = eval_operand src1 s1.state in
-          let v12 = eval_operand src2 s1.state in
-          let v21 = eval_operand src1 s2.state in
-          let v22 = eval_operand src2 s2.state in
-          let v1 = FStar.UInt.mul_mod #64 v11 v12 in
-          let v2 = FStar.UInt.mul_mod #64 v21 v22 in
-          if not (valid_mem64 ptr1 s1.state.mem) || not (valid_mem64 ptr2 s2.state.mem) then ()
-          else begin
-           lemma_store_load_mem64 ptr1 v1 s1.state.mem;
-          lemma_store_load_mem64 ptr2 v2 s2.state.mem;
-          lemma_valid_store_mem64 ptr1 v1 s1.state.mem;
-          lemma_valid_store_mem64 ptr2 v2 s2.state.mem;
-          lemma_frame_store_mem64 ptr1 v1 s1.state.mem;
-          lemma_frame_store_mem64 ptr2 v2 s2.state.mem
-          end
-
-val lemma_and_same_public: (ts:taintState) -> (ins:tainted_ins{let i, _, _ = ins.ops in S.And64? i}) -> (s1:traceState) -> (s2:traceState) -> (fuel:nat) -> Lemma
-(let b, ts' = check_if_ins_consumes_fixed_time ins ts in
-  (b2t b ==> isExplicitLeakageFreeGivenStates (Ins ins) fuel ts ts' s1 s2))
-
-let lemma_and_same_public ts ins s1 s2 fuel =
-  let b, ts' = check_if_ins_consumes_fixed_time ins ts in
-  let i, dsts, srcs = ins.ops in
-  let r1 = taint_eval_ins ins s1 in
-  let r2 = taint_eval_ins ins s2 in
-  match dsts with
-    | [OConst _] -> ()
-    | [OReg _] ->  ()
-    | [OMem m] ->
-      let ptr1 = eval_maddr m s1.state in
-      let ptr2 = eval_maddr m s2.state in
-      match srcs with
-        | [src1; src2] ->
-          let v11 = eval_operand src1 s1.state in
-          let v12 = eval_operand src2 s1.state in
-          let v21 = eval_operand src1 s2.state in
-          let v22 = eval_operand src2 s2.state in
-          let v1 = Types_s.iand v11 v12 in
-          let v2 = Types_s.iand v21 v22 in
-          if not (valid_mem64 ptr1 s1.state.mem) || not (valid_mem64 ptr2 s2.state.mem) then ()
-          else begin
-           lemma_store_load_mem64 ptr1 v1 s1.state.mem;
-          lemma_store_load_mem64 ptr2 v2 s2.state.mem;
-          lemma_valid_store_mem64 ptr1 v1 s1.state.mem;
-          lemma_valid_store_mem64 ptr2 v2 s2.state.mem;
-          lemma_frame_store_mem64 ptr1 v1 s1.state.mem;
-          lemma_frame_store_mem64 ptr2 v2 s2.state.mem
-          end
-
-val lemma_addlea_same_public: (ts:taintState) -> (ins:tainted_ins{let i, _, _ = ins.ops in S.AddLea64? i}) -> (s1:traceState) -> (s2:traceState) -> (fuel:nat) -> Lemma
-(let b, ts' = check_if_ins_consumes_fixed_time ins ts in
-  (b2t b ==> isExplicitLeakageFreeGivenStates (Ins ins) fuel ts ts' s1 s2))
-
-let lemma_addlea_same_public ts ins s1 s2 fuel =
-  let b, ts' = check_if_ins_consumes_fixed_time ins ts in
-  let i, dsts, srcs = ins.ops in
-  let r1 = taint_eval_ins ins s1 in
-  let r2 = taint_eval_ins ins s2 in
-  match dsts with
-    | [OConst _] -> ()
-    | [OReg _] ->  ()
-    | [OMem m] ->
-      let ptr1 = eval_maddr m s1.state in
-      let ptr2 = eval_maddr m s2.state in
-      match srcs with
-        | [dst; src1; src2] ->
-          let v11 = eval_operand src1 s1.state in
-          let v12 = eval_operand src2 s1.state in
-          let v21 = eval_operand src1 s2.state in
-          let v22 = eval_operand src2 s2.state in
-          let v1 = (v11 + v12) % pow2_64 in
-          let v2 = (v21 + v22) % pow2_64 in
-          if not (valid_mem64 ptr1 s1.state.mem) || not (valid_mem64 ptr2 s2.state.mem) then ()
-          else begin
-           lemma_store_load_mem64 ptr1 v1 s1.state.mem;
-          lemma_store_load_mem64 ptr2 v2 s2.state.mem;
-          lemma_valid_store_mem64 ptr1 v1 s1.state.mem;
-          lemma_valid_store_mem64 ptr2 v2 s2.state.mem;
-          lemma_frame_store_mem64 ptr1 v1 s1.state.mem;
-          lemma_frame_store_mem64 ptr2 v2 s2.state.mem
-          end
-
-val lemma_addcarry_same_public: (ts:taintState) -> (ins:tainted_ins{let i, _, _ = ins.ops in S.AddCarry64? i}) -> (s1:traceState) -> (s2:traceState) -> (fuel:nat) -> Lemma
-(let b, ts' = check_if_ins_consumes_fixed_time ins ts in
-  (b2t b ==> isExplicitLeakageFreeGivenStates (Ins ins) fuel ts ts' s1 s2))
-
-let lemma_addcarry_same_public ts ins s1 s2 fuel =
-  let b, ts' = check_if_ins_consumes_fixed_time ins ts in
-  let i, dsts, srcs = ins.ops in
-  let r1 = taint_eval_ins ins s1 in
-  let r2 = taint_eval_ins ins s2 in
-  match dsts with
-    | [OConst _] -> ()
-    | [OReg _] ->  ()
-    | [OMem m] ->
-      let ptr1 = eval_maddr m s1.state in
-      let ptr2 = eval_maddr m s2.state in
-      match srcs with
-        | [src1; src2] ->
-          let c1 = if cf(s1.state.X64.Memory_s.state.S.flags) then 1 else 0 in
-          let c2 = if cf(s2.state.X64.Memory_s.state.S.flags) then 1 else 0 in
-          let v11 = eval_operand src1 s1.state in
-          let v12 = eval_operand src2 s1.state in
-          let v21 = eval_operand src1 s2.state in
-          let v22 = eval_operand src2 s2.state in
-          let v1 = (v11 + v12 + c1) % pow2_64 in
-          let v2 = (v21 + v22 + c2) % pow2_64 in
-          if not (valid_mem64 ptr1 s1.state.mem) || not (valid_mem64 ptr2 s2.state.mem) then ()
-          else begin
-           lemma_store_load_mem64 ptr1 v1 s1.state.mem;
-          lemma_store_load_mem64 ptr2 v2 s2.state.mem;
-          lemma_valid_store_mem64 ptr1 v1 s1.state.mem;
-          lemma_valid_store_mem64 ptr2 v2 s2.state.mem;
-          lemma_frame_store_mem64 ptr1 v1 s1.state.mem;
-          lemma_frame_store_mem64 ptr2 v2 s2.state.mem
-          end
-
-val lemma_adcx_same_public: (ts:taintState) -> (ins:tainted_ins{let i, _, _ = ins.ops in S.Adcx64? i}) -> (s1:traceState) -> (s2:traceState) -> (fuel:nat) -> Lemma
-(let b, ts' = check_if_ins_consumes_fixed_time ins ts in
-  (b2t b ==> isExplicitLeakageFreeGivenStates (Ins ins) fuel ts ts' s1 s2))
-
-#reset-options "--initial_ifuel 2 --max_ifuel 2 --initial_fuel 4 --max_fuel 4 --z3rlimit 200"
-
-let lemma_adcx_same_public ts ins s1 s2 fuel =
-  let b, ts' = check_if_ins_consumes_fixed_time ins ts in
-  let i, dsts, srcs = ins.ops in
-  let r1 = taint_eval_ins ins s1 in
-  let r2 = taint_eval_ins ins s2 in
-  match dsts with
-    | [OConst _] -> ()
-    | [OReg _] ->  ()
-    | [OMem m] ->
-      let ptr1 = eval_maddr m s1.state in
-      let ptr2 = eval_maddr m s2.state in
-      match srcs with
-        | [src1; src2] ->
-          let c1 = if cf(s1.state.X64.Memory_s.state.S.flags) then 1 else 0 in
-          let c2 = if cf(s2.state.X64.Memory_s.state.S.flags) then 1 else 0 in
-          let v11 = eval_operand src1 s1.state in
-          let v12 = eval_operand src2 s1.state in
-          let v21 = eval_operand src1 s2.state in
-          let v22 = eval_operand src2 s2.state in
-          let v1 = (v11 + v12 + c1) % pow2_64 in
-          let v2 = (v21 + v22 + c2) % pow2_64 in
-          if not (valid_mem64 ptr1 s1.state.mem) || not (valid_mem64 ptr2 s2.state.mem) then ()
-          else begin
-           lemma_store_load_mem64 ptr1 v1 s1.state.mem;
-          lemma_store_load_mem64 ptr2 v2 s2.state.mem;
-          lemma_valid_store_mem64 ptr1 v1 s1.state.mem;
-          lemma_valid_store_mem64 ptr2 v2 s2.state.mem;
-          lemma_frame_store_mem64 ptr1 v1 s1.state.mem;
-          lemma_frame_store_mem64 ptr2 v2 s2.state.mem
-          end
-
-val lemma_mul_same_public: (ts:taintState) -> (ins:tainted_ins{let i, _, _ = ins.ops in S.Mul64? i}) -> (s1:traceState) -> (s2:traceState) -> (fuel:nat) -> Lemma
-(let b, ts' = check_if_ins_consumes_fixed_time ins ts in
-  (b2t b ==> isExplicitLeakageFreeGivenStates (Ins ins) fuel ts ts' s1 s2))
-
-let lemma_mul_same_public ts ins s1 s2 fuel = lemma_public_flags_same ts ins; ()
-
-val lemma_shr_same_public: (ts:taintState) -> (ins:tainted_ins{let i, _, _ = ins.ops in S.Shr64? i}) -> (s1:traceState) -> (s2:traceState) -> (fuel:nat) -> Lemma
-(let b, ts' = check_if_ins_consumes_fixed_time ins ts in
-  (b2t b ==> isExplicitLeakageFreeGivenStates (Ins ins) fuel ts ts' s1 s2))
-
-let lemma_shr_same_public ts ins s1 s2 fuel =
-  let b, ts' = check_if_ins_consumes_fixed_time ins ts in
-  let i, dsts, srcs = ins.ops in
-  let r1 = taint_eval_ins ins s1 in
-  let r2 = taint_eval_ins ins s2 in
-  match dsts with
-    | [OConst _] -> ()
-    | [OReg _] ->  ()
-    | [OMem m] ->
-      let ptr1 = eval_maddr m s1.state in
-      let ptr2 = eval_maddr m s2.state in
-      match srcs with
-        | [src1; src2] ->
-          let v11 = eval_operand src1 s1.state in
-          let v12 = eval_operand src2 s1.state in
-          let v21 = eval_operand src1 s2.state in
-          let v22 = eval_operand src2 s2.state in
-          let v1 = Types_s.ishr v11 v12 in
-          let v2 = Types_s.ishr v21 v22 in
-          if not (valid_mem64 ptr1 s1.state.mem) || not (valid_mem64 ptr2 s2.state.mem) then ()
-          else begin
-           lemma_store_load_mem64 ptr1 v1 s1.state.mem;
-          lemma_store_load_mem64 ptr2 v2 s2.state.mem;
-          lemma_valid_store_mem64 ptr1 v1 s1.state.mem;
-          lemma_valid_store_mem64 ptr2 v2 s2.state.mem;
-          lemma_frame_store_mem64 ptr1 v1 s1.state.mem;
-          lemma_frame_store_mem64 ptr2 v2 s2.state.mem
-          end
-
-val lemma_shl_same_public: (ts:taintState) -> (ins:tainted_ins{let i, _, _ = ins.ops in S.Shl64? i}) -> (s1:traceState) -> (s2:traceState) -> (fuel:nat) -> Lemma
-(let b, ts' = check_if_ins_consumes_fixed_time ins ts in
-  (b2t b ==> isExplicitLeakageFreeGivenStates (Ins ins) fuel ts ts' s1 s2))
-
-let lemma_shl_same_public ts ins s1 s2 fuel =
-  let b, ts' = check_if_ins_consumes_fixed_time ins ts in
-  let i, dsts, srcs = ins.ops in
-  let r1 = taint_eval_ins ins s1 in
-  let r2 = taint_eval_ins ins s2 in
-  match dsts with
-    | [OConst _] -> ()
-    | [OReg _] ->  ()
-    | [OMem m] ->
-      let ptr1 = eval_maddr m s1.state in
-      let ptr2 = eval_maddr m s2.state in
-      match srcs with
-        | [src1; src2] ->
-          let v11 = eval_operand src1 s1.state in
-          let v12 = eval_operand src2 s1.state in
-          let v21 = eval_operand src1 s2.state in
-          let v22 = eval_operand src2 s2.state in
-          let v1 = Types_s.ishl v11 v12 in
-          let v2 = Types_s.ishl v21 v22 in
-          if not (valid_mem64 ptr1 s1.state.mem) || not (valid_mem64 ptr2 s2.state.mem) then ()
-          else begin
-           lemma_store_load_mem64 ptr1 v1 s1.state.mem;
-          lemma_store_load_mem64 ptr2 v2 s2.state.mem;
-          lemma_valid_store_mem64 ptr1 v1 s1.state.mem;
-          lemma_valid_store_mem64 ptr2 v2 s2.state.mem;
-          lemma_frame_store_mem64 ptr1 v1 s1.state.mem;
-          lemma_frame_store_mem64 ptr2 v2 s2.state.mem
-          end
-
-val lemma_xor_same_public: (ts:taintState) -> (ins:tainted_ins{let i, _, _ = ins.ops in S.Xor64? i}) -> (s1:traceState) -> (s2:traceState) -> (fuel:nat) -> Lemma
-(let b, ts' = check_if_ins_consumes_fixed_time ins ts in
-  (b2t b ==> isExplicitLeakageFreeGivenStates (Ins ins) fuel ts ts' s1 s2))
+  = let b, ts' = check_if_ins_consumes_fixed_time ins ts in
+    Classical.move_requires (lemma_imul_same_public_aux ts ins s1 s2 fuel b) ts'
 
 val lemma_aux_xor: (x:nat64) -> Lemma (Types_s.ixor x x = 0)
 
@@ -613,43 +857,285 @@ let lemma_aux_xor x =
   TypesNative_s.reveal_ixor 64 x x;
   FStar.UInt.logxor_self #64 x
 
-let lemma_xor_same_public ts ins s1 s2 fuel =
-  let b, ts' = check_if_ins_consumes_fixed_time ins ts in
-  let i, dsts, srcs = ins.ops in
-  let r1 = taint_eval_ins ins s1 in
-  let r2 = taint_eval_ins ins s2 in
-  Classical.forall_intro lemma_aux_xor;
-  match dsts with
-    | [OConst _] -> ()
-    | [OReg _] -> ()
-    | [OMem m] ->
-      let ptr1 = eval_maddr m s1.state in
-      let ptr2 = eval_maddr m s2.state in
-      match srcs with
-        | [src1; src2] ->
-          let v11 = eval_operand src1 s1.state in
-          let v12 = eval_operand src2 s1.state in
-          let v21 = eval_operand src1 s2.state in
-          let v22 = eval_operand src2 s2.state in
-          let v1 = Types_s.ixor v11 v12 in
-          let v2 = Types_s.ixor v21 v22 in
-          if not (valid_mem64 ptr1 s1.state.mem) || not (valid_mem64 ptr2 s2.state.mem) then ()
-          else begin
-           lemma_store_load_mem64 ptr1 v1 s1.state.mem;
-          lemma_store_load_mem64 ptr2 v2 s2.state.mem;
-          lemma_valid_store_mem64 ptr1 v1 s1.state.mem;
-          lemma_valid_store_mem64 ptr2 v2 s2.state.mem;
-          lemma_frame_store_mem64 ptr1 v1 s1.state.mem;
-          lemma_frame_store_mem64 ptr2 v2 s2.state.mem
-          end
+let lemma_xor_same_public_aux (ts:taintState) (ins:tainted_ins{S.Xor64? ins.i}) (s1:traceState) (s2:traceState)
+                               (fuel:nat) (b:bool) (ts':taintState)
+  :Lemma (requires ((b, ts') == check_if_ins_consumes_fixed_time ins ts /\ b /\
+                    is_explicit_leakage_free_lhs (Ins ins) fuel ts ts' s1 s2))
+         (ensures  (is_explicit_leakage_free_rhs (Ins ins) fuel ts ts' s1 s2)) =
+    let S.Xor64 dst src, t = ins.i, ins.t in
+    let dsts, srcs = extract_operands ins.i in
+
+    Classical.forall_intro lemma_aux_xor;
+
+    let r1 = taint_eval_code (Ins ins) fuel s1 in
+    let r2 = taint_eval_code (Ins ins) fuel s2 in
+
+    let s1' = Some?.v r1 in
+    let s2' = Some?.v r2 in
+
+    let s1b = S.run (S.check (taint_match_list srcs t s1.memTaint)) s1.state in
+    let s2b = S.run (S.check (taint_match_list srcs t s2.memTaint)) s2.state in
+
+    let taint = sources_taint srcs ts ins.t in
+
+    let v11 = S.eval_operand dst s1.state in
+    let v12 = S.eval_operand src s1.state in
+    let v21 = S.eval_operand dst s2.state in
+    let v22 = S.eval_operand src s2.state in
+    let v1 = Types_s.ixor v11 v12 in
+    let v2 = Types_s.ixor v21 v22 in
+
+    let aux_value () : Lemma 
+      (requires Public? taint)
+      (ensures v1 == v2) = 
+      Opaque_s.reveal_opaque S.get_heap_val64_def 
+    in
+
+    match dst with
+    | OConst _ -> ()
+    | OReg r -> if Secret? taint then () else aux_value()
+    | OMem m -> begin
+      let aux (x:int) : Lemma
+        (requires Public? s1'.memTaint.[x] || Public? s2'.memTaint.[x])
+        (ensures s1'.state.S.mem.[x] == s2'.state.S.mem.[x]) =
+        let ptr1 = S.eval_maddr m s1.state in
+        let ptr2 = S.eval_maddr m s2.state in
+        assert (ptr1 == ptr2);
+         if x < ptr1 || x >= ptr1 + 8 then (
+          // If we're outside the modified area, nothing changed, the property still holds
+          frame_update_heap_x ptr1 x v1 s1b.S.mem;
+          frame_update_heap_x ptr1 x v2 s2b.S.mem
+        ) else (
+          if Secret? taint then ()
+          else (
+            aux_value();
+            correct_update_get ptr1 v1 s1b.S.mem;
+            correct_update_get ptr1 v2 s2b.S.mem;
+            // If values are identical, the bytes also are identical
+            same_mem_get_heap_val ptr1 s1'.state.S.mem s2'.state.S.mem
+          )
+        )
+      
+      in Classical.forall_intro (Classical.move_requires aux)
+    end
+
+let lemma_xor_same_public (ts:taintState) (ins:tainted_ins{S.Xor64? ins.i}) (s1:traceState) (s2:traceState) 
+  (fuel:nat)
+  :Lemma (let b, ts' = check_if_ins_consumes_fixed_time ins ts in
+  (b2t b ==> isExplicitLeakageFreeGivenStates (Ins ins) fuel ts ts' s1 s2))
+  = let b, ts' = check_if_ins_consumes_fixed_time ins ts in
+    Classical.move_requires (lemma_xor_same_public_aux ts ins s1 s2 fuel b) ts'
+
+
+let lemma_and_same_public_aux (ts:taintState) (ins:tainted_ins{S.And64? ins.i}) (s1:traceState) (s2:traceState)
+                               (fuel:nat) (b:bool) (ts':taintState)
+  :Lemma (requires ((b, ts') == check_if_ins_consumes_fixed_time ins ts /\ b /\
+                    is_explicit_leakage_free_lhs (Ins ins) fuel ts ts' s1 s2))
+         (ensures  (is_explicit_leakage_free_rhs (Ins ins) fuel ts ts' s1 s2)) =
+    let S.And64 dst src, t = ins.i, ins.t in
+    let dsts, srcs = extract_operands ins.i in
+
+    let r1 = taint_eval_code (Ins ins) fuel s1 in
+    let r2 = taint_eval_code (Ins ins) fuel s2 in
+
+    let s1' = Some?.v r1 in
+    let s2' = Some?.v r2 in
+
+    let s1b = S.run (S.check (taint_match_list srcs t s1.memTaint)) s1.state in
+    let s2b = S.run (S.check (taint_match_list srcs t s2.memTaint)) s2.state in
+
+    let taint = sources_taint srcs ts ins.t in
+
+    let v11 = S.eval_operand dst s1.state in
+    let v12 = S.eval_operand src s1.state in
+    let v21 = S.eval_operand dst s2.state in
+    let v22 = S.eval_operand src s2.state in
+    let v1 = Types_s.iand v11 v12 in
+    let v2 = Types_s.iand v21 v22 in
+
+    let aux_value () : Lemma 
+      (requires Public? taint)
+      (ensures v1 == v2) = 
+      Opaque_s.reveal_opaque S.get_heap_val64_def 
+    in
+
+    match dst with
+    | OConst _ -> ()
+    | OReg r -> if Secret? taint then () else aux_value()
+    | OMem m -> begin
+      let aux (x:int) : Lemma
+        (requires Public? s1'.memTaint.[x] || Public? s2'.memTaint.[x])
+        (ensures s1'.state.S.mem.[x] == s2'.state.S.mem.[x]) =
+        let ptr1 = S.eval_maddr m s1.state in
+        let ptr2 = S.eval_maddr m s2.state in
+        assert (ptr1 == ptr2);
+         if x < ptr1 || x >= ptr1 + 8 then (
+          // If we're outside the modified area, nothing changed, the property still holds
+          frame_update_heap_x ptr1 x v1 s1b.S.mem;
+          frame_update_heap_x ptr1 x v2 s2b.S.mem
+        ) else (
+          if Secret? taint then ()
+          else (
+            aux_value();
+            correct_update_get ptr1 v1 s1b.S.mem;
+            correct_update_get ptr1 v2 s2b.S.mem;
+            // If values are identical, the bytes also are identical
+            same_mem_get_heap_val ptr1 s1'.state.S.mem s2'.state.S.mem
+          )
+        )
+      
+      in Classical.forall_intro (Classical.move_requires aux)
+    end
+
+let lemma_and_same_public (ts:taintState) (ins:tainted_ins{S.And64? ins.i}) (s1:traceState) (s2:traceState) 
+  (fuel:nat)
+  :Lemma (let b, ts' = check_if_ins_consumes_fixed_time ins ts in
+  (b2t b ==> isExplicitLeakageFreeGivenStates (Ins ins) fuel ts ts' s1 s2))
+  = let b, ts' = check_if_ins_consumes_fixed_time ins ts in
+    Classical.move_requires (lemma_and_same_public_aux ts ins s1 s2 fuel b) ts'
+
+let lemma_shr_same_public_aux (ts:taintState) (ins:tainted_ins{S.Shr64? ins.i}) (s1:traceState) (s2:traceState)
+                               (fuel:nat) (b:bool) (ts':taintState)
+  :Lemma (requires ((b, ts') == check_if_ins_consumes_fixed_time ins ts /\ b /\
+                    is_explicit_leakage_free_lhs (Ins ins) fuel ts ts' s1 s2))
+         (ensures  (is_explicit_leakage_free_rhs (Ins ins) fuel ts ts' s1 s2)) =
+    let S.Shr64 dst src, t = ins.i, ins.t in
+    let dsts, srcs = extract_operands ins.i in
+
+    let r1 = taint_eval_code (Ins ins) fuel s1 in
+    let r2 = taint_eval_code (Ins ins) fuel s2 in
+
+    let s1' = Some?.v r1 in
+    let s2' = Some?.v r2 in
+
+    let s1b = S.run (S.check (taint_match_list srcs t s1.memTaint)) s1.state in
+    let s2b = S.run (S.check (taint_match_list srcs t s2.memTaint)) s2.state in
+
+    let taint = sources_taint srcs ts ins.t in
+
+    let v11 = S.eval_operand dst s1.state in
+    let v12 = S.eval_operand src s1.state in
+    let v21 = S.eval_operand dst s2.state in
+    let v22 = S.eval_operand src s2.state in
+    let v1 = Types_s.ishr v11 v12 in
+    let v2 = Types_s.ishr v21 v22 in
+
+    let aux_value () : Lemma 
+      (requires Public? taint)
+      (ensures v1 == v2) = 
+      Opaque_s.reveal_opaque S.get_heap_val64_def 
+    in
+
+    match dst with
+    | OConst _ -> ()
+    | OReg r -> if Secret? taint then () else aux_value()
+    | OMem m -> begin
+      let aux (x:int) : Lemma
+        (requires Public? s1'.memTaint.[x] || Public? s2'.memTaint.[x])
+        (ensures s1'.state.S.mem.[x] == s2'.state.S.mem.[x]) =
+        let ptr1 = S.eval_maddr m s1.state in
+        let ptr2 = S.eval_maddr m s2.state in
+        assert (ptr1 == ptr2);
+         if x < ptr1 || x >= ptr1 + 8 then (
+          // If we're outside the modified area, nothing changed, the property still holds
+          frame_update_heap_x ptr1 x v1 s1b.S.mem;
+          frame_update_heap_x ptr1 x v2 s2b.S.mem
+        ) else (
+          if Secret? taint then ()
+          else (
+            aux_value();
+            correct_update_get ptr1 v1 s1b.S.mem;
+            correct_update_get ptr1 v2 s2b.S.mem;
+            // If values are identical, the bytes also are identical
+            same_mem_get_heap_val ptr1 s1'.state.S.mem s2'.state.S.mem
+          )
+        )
+      
+      in Classical.forall_intro (Classical.move_requires aux)
+    end
+
+let lemma_shr_same_public (ts:taintState) (ins:tainted_ins{S.Shr64? ins.i}) (s1:traceState) (s2:traceState) 
+  (fuel:nat)
+  :Lemma (let b, ts' = check_if_ins_consumes_fixed_time ins ts in
+  (b2t b ==> isExplicitLeakageFreeGivenStates (Ins ins) fuel ts ts' s1 s2))
+  = let b, ts' = check_if_ins_consumes_fixed_time ins ts in
+    Classical.move_requires (lemma_shr_same_public_aux ts ins s1 s2 fuel b) ts'
+
+let lemma_shl_same_public_aux (ts:taintState) (ins:tainted_ins{S.Shl64? ins.i}) (s1:traceState) (s2:traceState)
+                               (fuel:nat) (b:bool) (ts':taintState)
+  :Lemma (requires ((b, ts') == check_if_ins_consumes_fixed_time ins ts /\ b /\
+                    is_explicit_leakage_free_lhs (Ins ins) fuel ts ts' s1 s2))
+         (ensures  (is_explicit_leakage_free_rhs (Ins ins) fuel ts ts' s1 s2)) =
+    let S.Shl64 dst src, t = ins.i, ins.t in
+    let dsts, srcs = extract_operands ins.i in
+
+    let r1 = taint_eval_code (Ins ins) fuel s1 in
+    let r2 = taint_eval_code (Ins ins) fuel s2 in
+
+    let s1' = Some?.v r1 in
+    let s2' = Some?.v r2 in
+
+    let s1b = S.run (S.check (taint_match_list srcs t s1.memTaint)) s1.state in
+    let s2b = S.run (S.check (taint_match_list srcs t s2.memTaint)) s2.state in
+
+    let taint = sources_taint srcs ts ins.t in
+
+    let v11 = S.eval_operand dst s1.state in
+    let v12 = S.eval_operand src s1.state in
+    let v21 = S.eval_operand dst s2.state in
+    let v22 = S.eval_operand src s2.state in
+    let v1 = Types_s.ishl v11 v12 in
+    let v2 = Types_s.ishl v21 v22 in
+
+    let aux_value () : Lemma 
+      (requires Public? taint)
+      (ensures v1 == v2) = 
+      Opaque_s.reveal_opaque S.get_heap_val64_def 
+    in
+
+    match dst with
+    | OConst _ -> ()
+    | OReg r -> if Secret? taint then () else aux_value()
+    | OMem m -> begin
+      let aux (x:int) : Lemma
+        (requires Public? s1'.memTaint.[x] || Public? s2'.memTaint.[x])
+        (ensures s1'.state.S.mem.[x] == s2'.state.S.mem.[x]) =
+        let ptr1 = S.eval_maddr m s1.state in
+        let ptr2 = S.eval_maddr m s2.state in
+        assert (ptr1 == ptr2);
+         if x < ptr1 || x >= ptr1 + 8 then (
+          // If we're outside the modified area, nothing changed, the property still holds
+          frame_update_heap_x ptr1 x v1 s1b.S.mem;
+          frame_update_heap_x ptr1 x v2 s2b.S.mem
+        ) else (
+          if Secret? taint then ()
+          else (
+            aux_value();
+            correct_update_get ptr1 v1 s1b.S.mem;
+            correct_update_get ptr1 v2 s2b.S.mem;
+            // If values are identical, the bytes also are identical
+            same_mem_get_heap_val ptr1 s1'.state.S.mem s2'.state.S.mem
+          )
+        )
+      
+      in Classical.forall_intro (Classical.move_requires aux)
+    end
+
+let lemma_shl_same_public (ts:taintState) (ins:tainted_ins{S.Shl64? ins.i}) (s1:traceState) (s2:traceState) 
+  (fuel:nat)
+  :Lemma (let b, ts' = check_if_ins_consumes_fixed_time ins ts in
+  (b2t b ==> isExplicitLeakageFreeGivenStates (Ins ins) fuel ts ts' s1 s2))
+  = let b, ts' = check_if_ins_consumes_fixed_time ins ts in
+    Classical.move_requires (lemma_shl_same_public_aux ts ins s1 s2 fuel b) ts'
 
 #reset-options "--initial_ifuel 2 --max_ifuel 2 --initial_fuel 4 --max_fuel 4 --z3rlimit 20"
 val lemma_ins_same_public: (ts:taintState) -> (ins:tainted_ins{not (is_xmm_ins ins)}) -> (s1:traceState) -> (s2:traceState) -> (fuel:nat) -> Lemma
 (let b, ts' = check_if_ins_consumes_fixed_time ins ts in
   (b2t b ==> isExplicitLeakageFreeGivenStates (Ins ins) fuel ts ts' s1 s2))
 
-let lemma_ins_same_public ts ins s1 s2 fuel = let i, _, _ = ins.ops in
-  match i with
+let lemma_ins_same_public ts ins s1 s2 fuel =
+  match ins.i with
+  | S.Cpuid -> admit() // TODO
   | S.Mov64 _ _ -> lemma_mov_same_public ts ins s1 s2 fuel
   | S.Add64 _ _ -> lemma_add_same_public ts ins s1 s2 fuel
   | S.AddLea64 _ _ _ -> lemma_addlea_same_public ts ins s1 s2 fuel
@@ -657,7 +1143,7 @@ let lemma_ins_same_public ts ins s1 s2 fuel = let i, _, _ = ins.ops in
   | S.IMul64 _ _ -> lemma_imul_same_public ts ins s1 s2 fuel
   | S.And64 _ _ -> lemma_and_same_public ts ins s1 s2 fuel
   | S.Mul64 _ -> lemma_mul_same_public ts ins s1 s2 fuel
-  | S.Mulx64 _ _ _ -> lemma_mulx_same_public ts ins s1 s2 fuel
+  | S.Mulx64 _ _ _ -> lemma_mulx_same_public ts ins s1 s2 fuel // TODO
   | S.Xor64 _ _ -> lemma_xor_same_public ts ins s1 s2 fuel
   | S.AddCarry64 _ _ -> lemma_addcarry_same_public ts ins s1 s2 fuel
   | S.Adcx64 _ _ -> lemma_adcx_same_public ts ins s1 s2 fuel
@@ -665,7 +1151,7 @@ let lemma_ins_same_public ts ins s1 s2 fuel = let i, _, _ = ins.ops in
   | S.Shr64 _ _ -> lemma_shr_same_public ts ins s1 s2 fuel
   | S.Push _ -> lemma_push_same_public ts ins s1 s2 fuel
   | S.Pop _ -> lemma_pop_same_public ts ins s1 s2 fuel
-  | S.Adox64 _ _ -> ()
+  | S.Adox64 _ _ -> () // TODO
 
 let lemma_ins_leakage_free ts ins =
   let b, ts' = check_if_ins_consumes_fixed_time ins ts in
